Backup

project/relational_graph.v
@@ -8,7 +8,7 @@ Print relation.
     fun X => X -> Prop. *)
 
 Definition my_Finite_Type : (Ensemble nat) := 
-    fun X => (X = 0) \/ (X = 1) .
+    fun X => (X = 0) \/ (X = 1) \/ (X = 2) .
 
     
 Definition valid_cond {t : Type} (nodes : Ensemble t) (rel : relation t) : Type :=
@@ -29,12 +29,17 @@ Definition my_Basic_Graph : RG nat.
 Proof.
   refine ({|
     gr_nodes := my_Finite_Type;
-    gr_edges := (fun (A B : nat) => (A = 0) /\ (B = 1));
+    gr_edges := (fun (A B : nat) => ((A = 0) /\ (B = 1)) \/ 
+                                    ((A = 1) /\ (B = 2)));
     gr_valid := _
   |}).
   unfold valid_cond. intros. split; unfold my_Finite_Type.
-  - left. apply H.
-  - right. apply H.
+  - destruct H.
+    + left. apply H.
+    + right. left. apply H. 
+  - destruct H.
+    + right. left. apply H.
+    + right. right. apply H.
 Defined.
 
 
@@ -92,4 +97,99 @@ Proof.
         + apply H0.
 Qed.
 
+(* Defining Operations on RGs: *)
+
+
+Definition RG_addNode {A : Type} (node : A) (rg : RG A) : RG A.
+Proof.
+    refine {|
+        gr_nodes := fun a => node = a \/ rg.(gr_nodes) a;
+        gr_edges := rg.(gr_edges);
+        gr_valid := _
+    |}.    
+    unfold valid_cond. intros. split.
+    - pose proof rg.(gr_valid). unfold valid_cond in X. apply X in H. right. apply H.
+    - pose proof rg.(gr_valid). unfold valid_cond in X. apply X in H. right. apply H.
+Defined.
+
+Definition RG_addEdge {A : Type} (from to : A) (rg : RG A) : RG A.
+Proof.
+    refine {|
+        gr_nodes := fun a => (RG_addNode to (RG_addNode from rg)).(gr_nodes) a;
+        gr_edges := fun a1 a2 => (a1 = from /\ a2 = to) \/ rg.(gr_edges) a1 a2;
+        gr_valid := _
+    |}.    
+    unfold valid_cond. simpl. intros. split.
+    - destruct H.
+        + right. left. destruct H. auto.
+        + right. right. pose proof rg.(gr_valid). unfold valid_cond in X. apply X in H. apply H.
+    - destruct H.
+        + left. destruct H. auto.
+        + right. right. pose proof rg.(gr_valid). unfold valid_cond in X. apply X in H. apply H.
+Qed.
+
+(* Also removes all associated edges *)
+Definition RG_removeNode {A : Type} (node : A) (rg : RG A) : RG A.
+Proof.
+    refine {|
+        gr_nodes := fun a => node <> a /\ rg.(gr_nodes) a;
+        gr_edges := fun a1 a2 => node <> a1 /\ node <> a2 /\ rg.(gr_edges) a1 a2;
+        gr_valid := _
+    |}.    
+    unfold valid_cond. intros. split.
+    - split.
+        + apply H.
+        + destruct H as [? [? ?]]. pose proof rg.(gr_valid). unfold valid_cond in X. apply X in H1. apply H1.
+    - split.
+        + apply H.
+        + destruct H as [? [? ?]]. pose proof rg.(gr_valid). unfold valid_cond in X. apply X in H1. apply H1.
+Qed.
+
+
+(* Does not remove associated nodes *)
+Definition RG_removeEdge {A : Type} (from to : A) (rg : RG A) : RG A.
+Proof.
+    refine {|
+        gr_nodes := rg.(gr_nodes);
+        gr_edges := fun a1 a2 => from <> a1 /\ to <> a2 /\ rg.(gr_edges) a1 a2;
+        gr_valid := _
+    |}.    
+    unfold valid_cond. intros. destruct H as [? [? ?]]. split.
+    - pose proof rg.(gr_valid). unfold valid_cond in X. apply X in H1. apply H1.
+    - pose proof rg.(gr_valid). unfold valid_cond in X. apply X in H1. apply H1.
+Qed.
+
+
+
+Definition RG_getOutgoingEdges {A : Type} (node : A) (rg : RG A) : relation A :=
+    fun (a1 a2 : A) => rg.(gr_edges) a1 a2 /\ a1 = node.
+
+Definition RG_getIncomingEdges {A : Type} (node : A) (rg : RG A) : relation A :=
+    fun (a1 a2 : A) => rg.(gr_edges) a1 a2 /\ a2 = node.
+
+Definition RG_getIncidentEdges {A : Type} (node : A) (rg : RG A) : relation A :=
+    fun (a1 a2 : A) => (RG_getOutgoingEdges node rg) a1 a2 \/ (RG_getIncomingEdges node rg) a1 a2.
+
+(* There can also be variations of this, where you the the neighbor nodes and not just edges ... *)
+
+Require Import Coq.Relations.Relation_Operators.
+Definition RG_existsPath {A : Type} (node1 node2 : A) (rg : RG A) : Prop :=
+    clos_trans A rg.(gr_edges) node1 node2.
+
+(* 0 -> 1 -> 2 *)
+
+Example RG_existsPath_example : RG_existsPath 0 1 my_Basic_Graph.
+Proof.
+    compute. apply t_step. auto.
+Qed.
+
+(* 0 -> 1 -> 2 *)
+Example RG_existsPath_example' : RG_existsPath 0 2 my_Basic_Graph.
+Proof.
+    compute. apply (t_trans _ _ _ 1).
+    - apply t_step. auto.
+    - apply t_step. auto.
+Qed.
+
+(* Start implementing search *)
 
