project/inductive/IG_operations_as_RG.v
@@ -1,0 +1,58 @@
+Require Import String.
+Require Import Coq.Arith.Arith.
+Open Scope string_scope.
+
+Require Import List.
+Require Import Bool.
+Import ListNotations.
+
+Require Import Coq.Relations.Relation_Definitions.
+Require Import Coq.Sets.Ensembles.
+
+Require Import MyProject.project.relational_graph.
+
+(* Record RG (t : Type) := {
+    gr_nodes : Ensemble t;
+    gr_edges : relation t;
+    gr_valid : valid_cond gr_nodes gr_edges
+}. *)
+
+(* Record Context' (A B : Type) := {
+    labNodes : list (A * B);
+    labEdges : list (LEdge B)
+}.
+
+Record MContext' (A B : Type) := {
+    mcontext : option (Context' A B)
+}.
+
+Record Decomp'_RG (A B : Type) := {
+    mcontext' : MContext' A B;
+    rg_rest : RG A B
+}. *)
+
+Definition empty_RG {A : Type} : RG A.
+Proof.
+    refine ({|
+        gr_nodes := fun (a : A) => False;
+        gr_edges := fun (a b : A) => False;
+        gr_valid := _
+    |}).
+    compute. auto.
+Qed.
+
+Definition isEmpty_RG {A : Type} (g : RG A) : Prop :=
+    forall (a : A), g.(gr_nodes) a = False.
+
+(* This seems impossible, since one needs to "computationally read the RG", which Prop does not allow *)
+Fail Definition matsh_RG {A : Type} (g : RG A) (n : A) : (option (Ensemble A * Ensemble A) * RG A) :=
+    match g.(gr_nodes) n with
+        | True => (Some (g.(gr_nodes), g.(gr_nodes)), g)
+        | False => (None, g)
+    end.
+
+Definition mkGraph_RG {A B : Type} (nodes : list A) (edges : list (A * A)) : RG A.
+
+Definition labNodes_RG {A B : Type} (g : RG A) : list (A).
+
+
