project/inductive/basic/inductive_graph_basic.v
@@ -1,0 +1,397 @@
+Require Import String.
+Require Import Coq.Arith.Arith.
+Open Scope string_scope.
+Require Import Coq.Structures.OrdersTac.
+
+Require Import List.
+Require Import Bool.
+Import ListNotations.
+
+
+(* https://rocq-prover.org/doc/v8.9/stdlib/Coq.FSets.FMapList.html *)
+Require Import FSets.
+Require Import FMaps.
+Require Import OrderedTypeEx.
+
+Open Scope nat_scope.
+
+Definition Node := Nat_as_OT.t.
+
+
+
+Module NatMap := FMapList.Make(Nat_as_OT).
+
+Module WF := WFacts_fun Nat_as_OT NatMap. (* Library of useful lemmas about maps *)
+Module WP := WProperties_fun Nat_as_OT NatMap. (* More useful stuff about maps *)
+Print Module WF.
+Print Module WP.
+Check Nat_as_OT.lt. (*   : positive -> positive -> Prop *)
+
+Module NatSet := FSetList.Make(Nat_as_OT).
+Print FSetEqProperties.
+Module NatSetProperties := EqProperties(NatSet).
+
+
+
+Definition IG : Type :=
+  NatMap.t (NatSet.t * NatSet.t).
+
+
+(* Start defining functionality: *)
+Definition empty : IG :=
+  NatMap.empty (NatSet.t * NatSet.t).
+
+
+Definition isEmpty (x : IG) : bool :=
+  NatMap.is_empty x.
+
+Compute isEmpty empty.
+
+(* Here start the helper functions for "matsh" *)
+
+(* Applies a function to a map entry if it exists quickly *)
+Definition updateEntry (n : Node) (f : (NatSet.t * NatSet.t) -> (NatSet.t * NatSet.t)) (ig : IG) : IG :=
+  match NatMap.find n ig with
+    | Some v => NatMap.add n (f v) ig
+    | None => ig
+  end.
+
+
+Definition cleanUp' (n : Node) (froms tos : NatSet.t) (ig : IG) : IG :=
+  (* Loop over ingoing edges of removed node to update the outgoing of all of those to not have n anymore *)
+  let ig' := NatSet.fold (fun (elem : Node) (acc : IG) =>
+  updateEntry elem (fun '(currFroms, currTos) => (NatSet.remove n currFroms, currTos))
+    acc) tos ig in
+
+  (* Loop over outgoing edges of removed node to update the ingoing of all of those to not have n anymore *)
+  NatSet.fold (fun (elem : Node) (acc : IG) =>
+  updateEntry elem (fun '(currFroms, currTos) => (currFroms, NatSet.remove n currTos))
+    acc) froms ig'.
+  
+
+
+Definition cleanUp(n : Node) (context : (NatSet.t * NatSet.t)) (ig : IG) : IG :=
+  match context with | (froms, tos) =>
+    cleanUp' n froms tos (NatMap.remove n ig)
+  end.
+
+
+Definition matsh (n : Node) (ig : IG) : (option (NatSet.t * NatSet.t) * IG) :=
+  match NatMap.find n ig with
+    | None => (None, ig)
+    | Some context as sContext => (sContext, cleanUp n context ig) 
+  end.
+
+
+
+(* Here start the helper functions for "mkGraph" *)
+
+(* This is the "&" constructor, but it has to be defined as a function, since it is too advanced *)
+Definition add (n : Node) (fromsTos : (NatSet.t * NatSet.t)) (ig : IG) : IG :=
+  NatMap.add n fromsTos ig.
+
+
+
+Definition insNode (n : Node) (ig : IG) : IG :=
+  add n (NatSet.empty, NatSet.empty) ig.
+  
+
+Definition insNodes (nodes : list Node) (ig : IG) : IG :=
+  fold_right insNode ig nodes.
+
+
+(* If one of the nodes of the edge does not exist, nothing happens *)
+Definition insEdge (edge : (Node * Node)) (ig : IG) : IG :=
+match edge with
+  | (from, to) =>  if NatMap.mem from ig && NatMap.mem to ig then updateEntry from (fun '(froms, tos) => (froms, NatSet.add to tos))
+                (
+                  (* Now update the other side of the edge *)
+                  updateEntry to (fun '(froms, tos) => (NatSet.add from froms, tos))
+                  ig
+                ) else ig
+end.
+
+
+
+
+Definition insEdges (edges : list (Node * Node)) (ig : IG) : IG :=
+  fold_right insEdge ig edges.
+
+
+
+Definition mkGraph (nodes : list Node) (edges : list (Node * Node)) : IG :=
+  insEdges edges (insNodes nodes empty).
+
+
+ 
+Definition labNodes (ig : IG) : list Node :=
+  map fst (NatMap.elements ig).
+
+
+
+Definition showIG (ig : IG) :=
+  map (fun '(node, (froms, tos)) => (node, (NatSet.elements froms, NatSet.elements tos))) (NatMap.elements ig).
+  
+Definition showDecomp (decomp : (option (NatSet.t * NatSet.t) * IG)) :=
+  match decomp with
+    | (None, ig) => (None, showIG ig)
+    | (Some (froms, tos), ig) => (Some (NatSet.elements froms, NatSet.elements tos), showIG ig)
+  end.
+
+
+
+Compute showIG (mkGraph [1; 2; 3] [(1, 2); (2, 3); (3, 1)]).
+
+Definition myBasicGraph := mkGraph [1; 2; 3] [(1, 2); (2, 3); (3, 1)].
+
+(* Here come the tests for each defined function (that is in the graph class): *)
+
+Compute showIG empty.
+
+Compute isEmpty empty.
+Compute isEmpty myBasicGraph.
+
+Compute showDecomp (matsh 2 myBasicGraph).
+
+Compute showIG (mkGraph [1; 2; 3] [(1, 2); (2, 3); (3, 1)]).
+
+Compute labNodes myBasicGraph.
+
+
+
+
+(* Here, I try out various equational specifications of an IG: *)
+
+(* Block to derive useful conversion theorem "In_labNodes_is_InMap" *)
+
+(* This is from software foundations. Eventually, I will move this somewhere else *)
+Lemma eqb_reflect : forall x y, reflect (x = y) (x =? y).
+Proof.
+  intros x y. apply iff_reflect. symmetry.
+  apply Nat.eqb_eq.
+Qed.
+Lemma ltb_reflect : forall x y, reflect (x < y) (x <? y).
+Proof.
+  intros x y. apply iff_reflect. symmetry.
+  apply Nat.ltb_lt.
+Qed.
+Lemma leb_reflect : forall x y, reflect (x <= y) (x <=? y).
+Proof.
+  intros x y. apply iff_reflect. symmetry.
+  apply Nat.leb_le.
+Qed.
+
+Hint Resolve ltb_reflect leb_reflect eqb_reflect : bdestruct.
+Ltac bdestruct X :=
+  let H := fresh in let e := fresh "e" in
+   evar (e: Prop);
+   assert (H: reflect e X); subst e;
+    [ auto with bdestruct
+    | destruct H as [H|H];
+       [ | try first [apply not_lt in H | apply not_le in H]]].
+(* End from Software foundations *)
+
+Require Import Coq.micromega.Lia.
+
+Check InA.
+
+(* Helper lemma for converting an In (of a map) to an InA, which will eventually be turned to a NatMap.In (which has useful lemmas)  *)
+Lemma In_map_fst_InA : forall (A B: Type) (a : A) (l : list (A * B)),
+  In a (map fst l) <-> exists (a0 : B), InA (fun (x el : (A * B)) => x = el) (a, a0) l.
+Proof.
+  intros. induction l; simpl.
+  - split; intros.
+    + destruct H.
+    + destruct H. inversion H.
+  - split; intros.
+    + destruct H.
+      -- exists (snd a0). left. destruct a0. destruct H. simpl. reflexivity.
+      -- edestruct IHl. apply H0 in H. destruct H. exists x. apply InA_cons. right. assumption.
+    + destruct H. inversion H.
+      -- left. destruct a0. destruct H1. simpl. reflexivity.
+      -- right. apply IHl. exists x. assumption.
+Qed.  
+
+Require Import Coq.Logic.FunctionalExtensionality.
+Require Import Coq.Logic.PropExtensionality.
+
+(* Conversion from key equality from map to my own (simply written in a slightly different manner) *)
+Lemma In_conditions_same : (NatMap.eq_key_elt (elt:=NatSet.t * NatSet.t)) = (fun x el : Node * (NatSet.t * NatSet.t) => x = el).
+Proof.
+  unfold NatMap.eq_key_elt. unfold NatMap.Raw.PX.eqke.
+  apply functional_extensionality.
+  intros.
+  apply functional_extensionality.
+  intros.
+  destruct x, x0.
+  simpl.
+  apply propositional_extensionality.
+  split; intros.
+  - destruct H. subst. reflexivity.
+  - inversion H. auto.
+Qed.
+
+(* This is the most useful one for proving other statements.
+  Use it to convert from "use friendly" In- statements to "provable" NatMap.In- statements  *)
+Lemma In_labNodes_is_InMap : forall (x : Node) (ig : IG),
+  In x (labNodes ig) <-> NatMap.In x ig.
+Proof.
+  intros. unfold labNodes.
+  rewrite In_map_fst_InA.
+  pose proof (WF.elements_in_iff ig).
+  rewrite In_conditions_same in H.
+  specialize H with x.
+  symmetry.
+  assumption.
+Qed.
+
+
+(* Here start "meaningful statements" *)
+
+
+(* 5 statements on inserting (helpers for mkGraph): update, insEdge, insEdges, insNode, insNodes *)
+Lemma updateEntry_does_not_change_key_set : forall (n : Node) (f : NatSet.t * NatSet.t -> NatSet.t * NatSet.t) (ig : IG) (x : Node),
+  In x (labNodes (updateEntry n f ig)) <-> In x (labNodes ig).
+Proof.
+  intros. unfold updateEntry.
+  destruct (NatMap.find (elt:=NatSet.t * NatSet.t) n ig) eqn:isIn.
+  - rewrite In_labNodes_is_InMap. rewrite In_labNodes_is_InMap. rewrite WF.add_in_iff.
+    rewrite WF.in_find_iff. split.
+    + intros. destruct H.
+      -- rewrite <- H. rewrite isIn. unfold not. intros. discriminate H0.
+      -- assumption.
+    + intros. right. assumption.
+  - reflexivity.
+Qed.
+
+
+Lemma insEdge_does_not_add_node : forall (edge : (Node * Node)) (ig : IG) (x : Node),
+  In x (labNodes (insEdge edge ig)) <-> In x (labNodes ig).
+Proof.
+  intros. unfold insEdge. destruct edge.
+  destruct (NatMap.mem (elt:=NatSet.t * NatSet.t) n ig && NatMap.mem (elt:=NatSet.t * NatSet.t) n0 ig) eqn:H0.
+  - rewrite updateEntry_does_not_change_key_set.
+    rewrite updateEntry_does_not_change_key_set.
+    reflexivity.
+  - reflexivity.
+Qed.
+
+
+Lemma insEdges_does_not_add_nodes : forall (edges : list (Node * Node)) (ig : IG) (x : Node),
+  In x (labNodes (insEdges edges ig)) <-> In x (labNodes ig).
+Proof.
+  intros. simpl. induction edges.
+  - simpl. reflexivity.
+  - simpl. rewrite insEdge_does_not_add_node. rewrite IHedges. reflexivity.
+Qed. 
+
+
+Lemma insNode_any_ins_node : forall (node : Node) (ig : IG) (x : Node),
+  In x (labNodes (insNode node ig)) <-> In x (node :: labNodes ig).
+Proof.
+  intros. simpl. unfold insNode.
+  rewrite In_labNodes_is_InMap. rewrite WF.add_in_iff.
+  rewrite In_labNodes_is_InMap.
+  reflexivity.
+Qed.  
+
+
+Lemma insNodes_any_ins_all_nodes : forall (nodes : list Node) (ig : IG) (x : Node),
+  In x (labNodes (insNodes nodes ig)) <-> In x (nodes ++ labNodes ig).
+Proof.
+  intros. induction nodes.
+    - simpl. reflexivity.
+    - simpl. rewrite insNode_any_ins_node. simpl. rewrite IHnodes. reflexivity.
+Qed.
+
+
+(* "big" statements *)
+Theorem mkGraph_any_ins_all_nodes : forall (nl : list Node) (el : list (Node * Node)) (x : Node),
+  In x (labNodes (mkGraph nl el)) <-> In x nl.
+Proof.
+  intros. unfold mkGraph. rewrite insEdges_does_not_add_nodes. rewrite insNodes_any_ins_all_nodes.
+  rewrite app_nil_r. reflexivity.
+Qed.
+
+
+Theorem empty_isEmpty : isEmpty empty = true.
+Proof.
+  compute. reflexivity.
+Qed.
+
+Theorem labNodes_empty_nil : labNodes empty = [].
+Proof.
+  compute. reflexivity.
+Qed.
+
+
+(* Protipp: firstorder and congruence seem pretty useful *)
+Lemma not_NatMap_Empty_is_empty_false : forall (A : Type) (m : NatMap.t A), not (NatMap.Empty m) <-> NatMap.is_empty m = false.
+Proof.
+  intros. unfold not. rewrite WF.is_empty_iff. destruct (NatMap.is_empty (elt:=A) m) eqn:cond.
+  - firstorder. congruence.
+  - firstorder. congruence.
+Qed.
+
+(* Is probably also a <-> *)
+Theorem  non_empty_isEmpty_false : forall (nl : list Node) (el : list (Node * Node)),
+  length nl <> 0 -> isEmpty ((mkGraph nl el)) = false.
+Proof.
+  intros. destruct nl.
+  - simpl in H. destruct H. reflexivity.
+  - unfold isEmpty. apply not_NatMap_Empty_is_empty_false. unfold not. intros.
+    apply WP.elements_Empty in H0.
+    assert (HH : not (exists e, InA (fun x el : Node * (NatSet.t * NatSet.t) => x = el) (n, e) [])). {
+      unfold not. intros. destruct H1. inversion H1.
+    }
+
+    symmetry in H0. unfold not in HH. apply HH.
+
+    
+    rewrite H0 in HH.
+
+    rewrite <- In_conditions_same in HH.
+
+    apply HH.
+    pose proof WF.elements_in_iff.
+    edestruct H1.
+
+    apply H2.
+    apply In_labNodes_is_InMap.
+    apply mkGraph_any_ins_all_nodes. simpl. left. reflexivity.
+Qed.
+
+
+  (* intros. destruct nl; simpl.
+  - firstorder.
+    unfold isEmpty in H. apply not_NatMap_Empty_is_empty_false in H. rewrite WP.elements_Empty in H. unfold not in H.
+    exfalso.
+    apply H.
+    assert (HH : forall n, not (exists e, InA (fun x el : Node * (NatSet.t * NatSet.t) => x = el) (n, e) [])). {
+      unfold not. intros. destruct H0. inversion H0.
+    }
+    rewrite <- In_conditions_same in HH.
+  
+    pose proof WF.elements_in_iff.
+
+    assert (HH : not (exists e, InA (fun x el : NatMap.key * (NatSet.t * NatSet.t) => x = el) (n, e) [])). {
+      unfold not. intros. destruct H1. inversion H1.
+    } *)
+
+
+
+
+
+Theorem spec3 : forall (A B : Type) (n : Node), matsh n (empty) = (None, empty).
+Proof.
+  intros. compute.
+Admitted.
+
+Theorem spec4 : forall (A B : Type) (n : LNode A) (nl : list (LNode A)) (el : list (LEdge B)), 
+  In n nl -> exists map1 map2, matsh (fst n) (mkGraph nl el) =
+  (Some ((map1), snd n, (map2)), mkGraph (filter (fun '(idx, lab) => negb (fst n =? idx)) nl) (filter (fun '(to, from, lab) => negb ((to =? fst n) || (from =? fst n))) el)).
+(* This is not even a complete specification and it looks like a nightmare to prove... *)
+
+Theorem spec5 : forall (A B : Type) (n : LNode A) (nl : list (LNode A)) (el : list (LEdge B)), 
+  not (In n nl) -> matsh (fst n) (mkGraph nl el) = (None, mkGraph nl el).
+
